# 10.3
### **(a)**
 
$x = γ1 + θ1 z + v$  
$E(x) = γ1 + θ1 E(z)$  
$(x - E(x)) = θ1(z - E(z)) + v$  
$(z - E(z)) (x - E(x)) = θ1 ((z - E(z)) ^ 2) + (z - E(z)) v = θ1 ((z - E(z)) ^ 2)$  
$(z - E(z)) (x - E(x)) = θ1 ((z - E(z)) ^ 2)$  
$θ1 = (z - E(z)) (x - E(x)) / (z - E(z)) ^ 2$  


### **(b)**

$y = π0 + π1 z + u$  
$E(y) = π0 + π1 E(z)$  
$(y - E(y)) = π1(z - E(z)) + u$  
$(z - E(z)) (y - E(y)) = π1 ((z - E(z)) ^ 2) + (z - E(z)) u = π1 ((z - E(z)) ^ 2)$  
$(z - E(z)) (y - E(y)) = π1 ((z - E(z)) ^ 2)$  
$π1 = (z - E(z)) (y - E(y)) / (z - E(z)) ^ 2$  


### **(c)**

$$
\begin{align*}
y & = β1 + β2x + e = β1 + β2(γ1 + θ1z + v) + e\\
  & = β1 + β2γ1 + β2θ1z + β2v + e\\
  & = π0 + π1z + u
\end{align*}
$$

$π0 = β1 + β2γ1$  
$π1z = β2θ1z$ 
$π1 = β2θ1$  
$u = β2v + e$  


### **(d)**

$π1 = β2θ1$  
$β2 = π1 / θ1$  


### **(e)**
Using the Law of Large Numbers  
$\(\hat{\beta}_2 = \frac{\hat{\pi}_1}{\hat{\theta}_1}\)$
->
$\(\frac{\pi_1}{\theta_1}\ = \beta_2)$

