### 10.3 In the regression model $y = \beta_1+ \beta_2x + e$, assume $x$ is endogenous and that $z$ is a valid instrument. In Section 10.3.5, we saw that $\beta_2 = cov(z, y)∕cov(z, x)$.
---

#### a. Divide the denominator of $\beta_2 = cov(z, y)∕cov(z, x)$ by $var(z)$. Show that $cov(z, x)/var(z)$ is the coefficient of the simple regression with dependent variable $x$ and explanatory variable $z$, $x = \gamma_1 + \theta_1z + v$. [Hint: See Section 10.2.1.] Note that this is the first-stage equation in two-stage least squares.

Consider the **first-stage regression**: $x = \gamma_1 + \theta_1 z + v$

In simple linear regression, the slope estimate is: $\theta_1 = \frac{\text{cov}(z, x)}{\text{var}(z)}$ which is the slope coefficient from the first-stage regression of $x$ on $z$.

#### b. Divide the numerator of $\beta_2 = cov(z, y)∕cov(z, x)$ by $var(z)$. Show that $cov(z, y)/var(z)$ is the coefficient of a simple regression with dependent variable $y$ and explanatory variable $z$, $y = \pi_0 + \pi_1z + u$. [Hint: See Section 10.2.1.]

Consider the **reduced-form regression**: $y = \pi_0 + \pi_1 z + u$

The slope coefficient in this regression is: $\pi_1 = \frac{\text{cov}(z, y)}{\text{var}(z)}$ which is the slope from the reduced-form regression of $y$ on $z$.

#### c. In the model $y = \beta_1+ \beta_2x + e$, substitute for $x$ using $x = \gamma_1 + \theta_1z + v$ and simplify to obtain $y = \pi_0 + \pi_1z + u$. What are $\pi_0, \pi_1$, and $u$ in terms of the regression model parameters and error and the first-stage parameters and error? The regression you have obtained is a reduced-form equation.

Start with the structural equation: $y = \beta_1 + \beta_2 x + e$

Substitute the first-stage regression: $x = \gamma_1 + \theta_1 z + v$

Then: $y = \beta_1 + \beta_2 (\gamma_1 + \theta_1 z + v) + e \\ = \beta_1 + \beta_2 \gamma_1 + \beta_2 \theta_1 z + \beta_2 v + e$

Define:

- $\pi_0 = \beta_1 + \beta_2 \gamma_1$
- $\pi_1 = \beta_2 \theta_1$
- $u = \beta_2 v + e$

Thus, we obtain the reduced-form equation: $y = \pi_0 + \pi_1 z + u$

#### d. Show that $\beta_2 = \pi_1∕ \theta_1$.

#### e. If $\hat{\pi_1}$ and  $\hat{\theta_1}$ are the OLS estimators of $\pi_1$ and $\theta_1$, show that $\hat{\beta_2} = \hat{\pi_1} / \hat{\theta_1}$ is a consistent estimator of $\beta_2 = \pi_1∕ \theta_1$. The estimator $\hat{\beta_2} = \hat{\pi_1} / \hat{\theta_1}$ is an indirect least squares estimator.
