
### 1. set up  $X$, $Y$

```math
X = 
\begin{bmatrix}
1 & x_1 \\
1 & x_2 \\
\vdots & \vdots \\
1 & x_n
\end{bmatrix}_{n \times 2}, \quad
Y = 
\begin{bmatrix}
y_1 \\
\vdots \\
y_n
\end{bmatrix}_{n \times 1}
```

---

### 2. Substitute into the formula $\mathbf{b} = (X'X)^{-1}X'Y$

```math
X'X = 
\begin{bmatrix}
1 & \cdots & 1 \\
x_1 & \cdots & x_n
\end{bmatrix}
\begin{bmatrix}
1 & x_1 \\
\vdots & \vdots \\
1 & x_n
\end{bmatrix}
=
\begin{bmatrix}
n & \sum x_i \\
\sum x_i & \sum x_i^2
\end{bmatrix}
```

```math
X'Y = 
\begin{bmatrix}
1 & \cdots & 1 \\
x_1 & \cdots & x_n
\end{bmatrix}
\begin{bmatrix}
y_1 \\
\vdots \\
y_n
\end{bmatrix}
=
\begin{bmatrix}
\sum y_i \\
\sum x_i y_i
\end{bmatrix}
```

---

### 3. $\mathbf{b} = (X'X)^{-1}X'Y$

$$
(X'X)^{-1} = 
\frac{1}{n \sum x_i^2 - (\sum x_i)^2}
\begin{bmatrix}
\sum x_i^2 & -\sum x_i \\
-\sum x_i & n
\end{bmatrix}
$$

---

### 4. Multiply by $X'Y$

$$
\mathbf{b} = (X'X)^{-1}X'Y =
\frac{1}{n \sum x_i^2 - (\sum x_i)^2}
\begin{bmatrix}
\sum x_i^2 & -\sum x_i \\
-\sum x_i & n
\end{bmatrix}
\begin{bmatrix}
\sum y_i \\
\sum x_i y_i
\end{bmatrix}
$$

---

### 5. After expansion

Compute the slope term $b_2$

$$
b_2 = \frac{-\sum x_i \sum y_i + n \sum x_i y_i}{n \sum x_i^2 - (\sum x_i)^2}
$$

Substitute  $\bar{x} = \frac{1}{n} \sum x_i$, $\bar{y} = \frac{1}{n} \sum y_i$

$$
= \frac{-n \bar{x} \sum y_i + n \sum x_i y_i}{n \sum x_i^2 - n^2 \bar{x}^2}
= \frac{n \sum x_i y_i - n^2 \bar{x} \bar{y}}{n \sum x_i^2 - n^2 \bar{x}^2}
$$

$$
= \frac{\sum x_i y_i - n \bar{x} \bar{y}}{\sum x_i^2 - n \bar{x}^2}
= \frac{\sum (x_i - \bar{x})(y_i - \bar{y})}{\sum (x_i - \bar{x})^2} \tag{2.7}
$$

---

* Compute the intercept term $b_1$

$$
\begin{aligned}
b_1 &= \frac{\sum x_i^2 \sum y_i - \sum x_i \sum x_i y_i}{n \sum x_i^2 - (\sum x_i)^2} \\
    &= \frac{n \bar{y} \sum x_i^2 - \sum x_i \sum x_i y_i}{n \sum x_i^2 - (\sum x_i)^2} \\
    &= \bar{y} - b_2 \bar{x}
\end{aligned}
\tag{2.8}
$$

