313652028 鄭詠融 Martin

# 10.3(c) Substitute and Derive the Reduced-Form Equation

In the model $y = \beta_1 + \beta_2 x + e$, substitute for $x$ using $x = \gamma_1 + \theta_1 z + \nu$ and simplify to obtain $y = \pi_0 + \pi_1 z + u$.  
Identify $\pi_0$, $\pi_1$, and $u$ in terms of the regression model parameters and errors.

---

## Ans

Starting from the original structural equation:

$$
y = \beta_1 + \beta_2 x + e
$$

Substituting the expression for $x$:

$$
x = \gamma_1 + \theta_1 z + \nu
$$

we obtain:

$$
y = \beta_1 + \beta_2 (\gamma_1 + \theta_1 z + \nu) + e
$$

Expanding the terms:

$$
y = \beta_1 + \beta_2 \gamma_1 + \beta_2 \theta_1 z + \beta_2 \nu + e
$$

Group terms involving $z$ and the error terms:

$$
y = (\beta_1 + \beta_2 \gamma_1) + (\beta_2 \theta_1) z + (\beta_2 \nu + e)
$$

Comparing this with the reduced-form equation:

$$
y = \pi_0 + \pi_1 z + u
$$

we can identify:

- $\pi_0 = \beta_1 + \beta_2 \gamma_1$
- $\pi_1 = \beta_2 \theta_1$
- $u = \beta_2 \nu + e$

Thus, the reduced-form equation expresses $y$ directly as a function of the instrument $z$,  
with the composite error term $u$ absorbing the original structural error $e$ and the first-stage residual $\nu$.

