![image](https://github.com/user-attachments/assets/45b8c6db-49dc-48f1-909a-14b847f2be95)

We are given a regression model:  
**y = β₁ + β₂·x + e**,  
where `x` is endogenous and `z` is a valid instrument.

---

## (a) Denominator of β₂ = cov(z, y) / cov(z, x)

Divide the denominator by var(z):

    cov(z, x) / var(z)

This is the slope coefficient of the simple regression of `x` on `z`:

    x = γ₁ + θ₁·z + ν

→ Therefore, **θ₁ = cov(z, x) / var(z)**  
This is the **first-stage regression** in 2SLS.

---

## (b) Numerator of β₂ = cov(z, y) / cov(z, x)

Divide the numerator by var(z):

    cov(z, y) / var(z)

This is the slope coefficient of the simple regression of `y` on `z`:

    y = π₀ + π₁·z + u

→ Therefore, **π₁ = cov(z, y) / var(z)**

---

## (c) Derive the Reduced-Form Equation

Start from:

    y = β₁ + β₂·x + e

Substitute:

    x = γ₁ + θ₁·z + ν

Then:

    y = β₁ + β₂(γ₁ + θ₁·z + ν) + e  
      = (β₁ + β₂·γ₁) + β₂·θ₁·z + (β₂·ν + e)

Compare with:

    y = π₀ + π₁·z + u

We get:

- π₀ = β₁ + β₂·γ₁  
- π₁ = β₂·θ₁  
- u   = β₂·ν + e

This is the **reduced-form equation**.

---

## (d) Show that β₂ = π₁ / θ₁

From (c):  
π₁ = β₂·θ₁  
→ Solving for β₂:

    β₂ = π₁ / θ₁

---

## (e) Show that β̂₂ = π̂₁ / θ̂₁ is a consistent estimator of β₂

If:

- π̂₁ is the OLS estimator of π₁ (from regression y on z)
- θ̂₁ is the OLS estimator of θ₁ (from regression x on z)

Then:

    β̂₂ = π̂₁ / θ̂₁

By **Slutsky's theorem**, this ratio is a consistent estimator of:

    β₂ = π₁ / θ₁

Hence, **β̂₂ is the Indirect Least Squares (ILS) estimator** of β₂.
