# 2.1
## (a)
\[
\begin{array}{|c|c|c|c|c|c|}
\hline
(x) & (y) & (x - \bar{x}) & (x - \bar{x})^2 & (y - \bar{y}) & ( (x - \bar{x}) (y - \bar{y}) ) \\
\hline
3  & 4  & 2  & 4  & 1.6  & 3.2  \\
2  & 2  & 1  & 1  & -0.4  & -0.4  \\
1  & 3  & 0  & 0  & 0.6  & 0  \\
-1  & 1  & -2  & 4  & -1.4  & 2.8  \\
0  & 0  & -1  & 1  & -2.4  & 2.4  \\
\hline
\sum x_i = 5  & \sum y_i = 10  & \sum (x_i - \bar{x}) = 0  & \sum (x_i - \bar{x})^2 = 10  & \sum (y_i - \bar{y}) = 0  & \sum (x_i - \bar{x})(y_i - \bar{y}) = 8  \\
\hline
\end{array}
\]

## (b)
$$
b_2 = \frac{\sum (x_i - \bar{x}) (y_i - \bar{y})}{\sum (x_i - \bar{x})^2} = 
$$

$$
b_1 = \bar{y} - b_2 \bar{x} = 
$$
